Finish syntactic clos_mti proof for all but Letrec and Op
I'm now convinced this proof will work since everything to do with
non-recursive closures worked. Currently, Op is cheated and Letrec
is ruled out by a syntactic well-formedness check.

compiler/backend/proofs/clos_mtiProofScript.sml
@@ -1,5 +1,5 @@
 (* A proof of the clos_mti compiler pass. The theorem is proved using
-   a backwards simulation, i.e. against the direction of compilation. *) 
+   a backwards simulation, i.e. against the direction of compilation. *)
 open preamble; open closPropsTheory
 clos_mtiTheory closSemTheory;
 
@@ -12,61 +12,77 @@ val _ = bring_fwd_ctors "closLang" ``:closLang$exp``
 (* well-formed syntax *)
 
 val syntax_ok_def = tDefine "syntax_ok" `
-  (syntax_ok max_app [] <=> T) ∧
-  (syntax_ok max_app (e1::e2::es) <=>
-    syntax_ok max_app [e1] /\
-    syntax_ok max_app (e2::es)) /\
-  (syntax_ok max_app [Var t n] = T) ∧
-  (syntax_ok max_app [If t e1 e2 e3] <=>
-    syntax_ok max_app [e1] /\
-    syntax_ok max_app [e2] /\
-    syntax_ok max_app [e3]) ∧
-  (syntax_ok max_app [Let t es e] <=>
-    syntax_ok max_app es /\
-    syntax_ok max_app [e]) ∧
-  (syntax_ok max_app [Raise t e] <=>
-    syntax_ok max_app [e]) ∧
-  (syntax_ok max_app [Handle t e1 e2] <=>
-    syntax_ok max_app [e1] /\
-    syntax_ok max_app [e2]) ∧
-  (syntax_ok max_app [Tick t e] <=>
-    syntax_ok max_app [e]) ∧
-  (syntax_ok max_app [Call t ticks n es] = F) /\
-  (syntax_ok max_app [App t opt e es] <=>
+  (syntax_ok [] <=> T) ∧
+  (syntax_ok (e1::e2::es) <=>
+    syntax_ok [e1] /\
+    syntax_ok (e2::es)) /\
+  (syntax_ok [Var t n] = T) ∧
+  (syntax_ok [If t e1 e2 e3] <=>
+    syntax_ok [e1] /\
+    syntax_ok [e2] /\
+    syntax_ok [e3]) ∧
+  (syntax_ok [Let t es e] <=>
+    syntax_ok es /\
+    syntax_ok [e]) ∧
+  (syntax_ok [Raise t e] <=>
+    syntax_ok [e]) ∧
+  (syntax_ok [Handle t e1 e2] <=>
+    syntax_ok [e1] /\
+    syntax_ok [e2]) ∧
+  (syntax_ok [Tick t e] <=>
+    syntax_ok [e]) ∧
+  (syntax_ok [Call t ticks n es] = F) /\
+  (syntax_ok [App t opt e es] <=>
     LENGTH es = 1 /\ opt = NONE /\
-    syntax_ok max_app es /\
-    syntax_ok max_app [e]) ∧
-  (syntax_ok max_app [Fn t opt1 opt2 num_args e] <=>
+    syntax_ok es /\
+    syntax_ok [e]) ∧
+  (syntax_ok [Fn t opt1 opt2 num_args e] <=>
     num_args = 1 /\ opt1 = NONE /\ opt2 = NONE /\
-    syntax_ok max_app [e]) /\
-  (syntax_ok max_app [Letrec t _ _ funs e] <=> 
+    syntax_ok [e]) /\
+  (syntax_ok [Letrec t _ _ funs e] <=>
     F (* TODO: fix this *)) ∧
-  (syntax_ok max_app [Op t op es] <=>
-    syntax_ok max_app es)`
-  (WF_REL_TAC `measure (exp3_size o SND)`);
+  (syntax_ok [Op t op es] <=>
+    syntax_ok es)`
+  (WF_REL_TAC `measure exp3_size`);
+
+val syntax_ok_cons = store_thm("syntax_ok_cons",
+  ``syntax_ok (x::xs) <=> syntax_ok [x] /\ syntax_ok xs``,
+  Cases_on `xs` \\ fs [syntax_ok_def]);
+
+val syntax_ok_append = store_thm("syntax_ok_append[simp]",
+  ``!xs ys. syntax_ok (xs ++ ys) <=> syntax_ok xs /\ syntax_ok ys``,
+  Induct \\ fs [syntax_ok_def]
+  \\ once_rewrite_tac [syntax_ok_cons]
+  \\ fs [syntax_ok_def] \\ rw [] \\ eq_tac \\ rw[]);
 
 (* code relation *)
 
 val code_rel_def = Define `
   code_rel max_app e1 e2 <=>
-    syntax_ok max_app e1 /\ (e2 = intro_multi max_app e1)`
+    syntax_ok e1 /\ (e2 = intro_multi max_app e1)`
 
 val code_rel_IMP_LENGTH = store_thm("code_rel_IMP_LENGTH",
   ``code_rel max_app xs ys ==> LENGTH ys = LENGTH xs``,
   rw [code_rel_def,clos_mtiTheory.intro_multi_length]);
 
-val NEQ_intro_multi = store_thm("NEQ_intro_multi[simp]",
-  ``[Var loc_opt n] <> intro_multi max_app [App t o1 e1 l1] /\
-    [Var loc_opt n] <> intro_multi max_app [Fn t o0 o' n' e] /\
-    [Var loc_opt n] <> intro_multi max_app [Letrec t o0 o' l e] /\ 
-    [Fn v7 loc vsopt num_args exp] <> intro_multi max_app [App t o1 e1 l1] /\ 
-    [Fn v7 loc vsopt num_args exp] <> intro_multi max_app [Letrec t o0 o' l e]``,
-  cheat);
+val HD_intro_multi = store_thm("HD_intro_multi[simp]",
+  ``[HD (intro_multi max_app [e2])] = intro_multi max_app [e2]``,
+  `?x. intro_multi max_app [e2] = [x]` by metis_tac [intro_multi_sing]
+  \\ fs []);
+
+val intro_multi_cons = store_thm("intro_multi_cons",
+  ``!xs x. intro_multi m (x::xs) = HD (intro_multi m [x]) :: intro_multi m xs``,
+  Induct \\ fs[intro_multi_def]);
 
 val code_rel_CONS_CONS = store_thm("code_rel_CONS_CONS",
   ``code_rel m (x1::x2::xs) (y1::y2::ys) <=>
     code_rel m [x1] [y1] /\ code_rel m (x2::xs) (y2::ys)``,
-  cheat);  
+  fs [code_rel_def,syntax_ok_def,intro_multi_def]
+  \\ `?t1. intro_multi m [x1] = [t1]` by metis_tac [intro_multi_sing]
+  \\ `?t2. intro_multi m [x2] = [t2]` by metis_tac [intro_multi_sing]
+  \\ fs [] \\ eq_tac \\ rw []
+  \\ pop_assum mp_tac
+  \\ once_rewrite_tac [intro_multi_cons] \\ fs []);
 
 (* value relation *)
 
@@ -79,32 +95,33 @@ val (v_rel_rules, v_rel_ind, v_rel_cases) = Hol_reln `
   (!w. v_rel max_app (Word64 w) (Word64 w)) /\
   (!b. v_rel max_app (ByteVector w) (ByteVector b)) /\
   (!n. v_rel max_app (RefPtr n) (RefPtr n)) /\
-  (!tag xs ys. 
+  (!tag xs ys.
      LIST_REL (v_rel max_app) xs ys ==>
      v_rel max_app (Block tag xs) (Block tag ys)) /\
-  (!args env1 env2 arg_count e1 ts e2.
-     LENGTH ts + LENGTH args = arg_count /\
+  (!args1 args2 env1 env2 arg_count e1 ts e2.
+     1 + LENGTH ts + LENGTH args1 = arg_count /\
      code_rel max_app [e1] [e2] /\
      LIST_REL (v_rel max_app) env1 env2 /\
-     LENGTH args < arg_count ==>
-     v_rel max_app 
-       (Closure NONE [] (args ++ env1) 1 (mk_Fns ts e1))
-       (Closure NONE args env2 arg_count e2))
+     LIST_REL (v_rel max_app) args1 args2 /\
+     LENGTH args1 < arg_count ==>
+     v_rel max_app
+       (Closure NONE [] (args1 ++ env1) 1 (mk_Fns ts e1))
+       (Closure NONE args2 env2 arg_count e2))
   (* TODO: add case for Recclosure *)`
 
 val v_rel_opt_def = Define `
-  (v_rel_opt max_app NONE NONE <=> T) /\ 
+  (v_rel_opt max_app NONE NONE <=> T) /\
   (v_rel_opt max_app (SOME x) (SOME y) <=> v_rel max_app x y) /\
   (v_rel_opt max_app _ _ = F)`;
 
 val (ref_rel_rules, ref_rel_ind, ref_rel_cases) = Hol_reln `
   (!b bs. ref_rel max_app (ByteArray b bs) (ByteArray b bs)) /\
   (!xs ys.
-    LIST_REL (v_rel max_app) xs ys ==>    
+    LIST_REL (v_rel max_app) xs ys ==>
     ref_rel max_app (ValueArray xs) (ValueArray ys))`
 
 val FMAP_REL_def = Define `
-  FMAP_REL r f1 f2 <=> 
+  FMAP_REL r f1 f2 <=>
     FDOM f1 = FDOM f2 /\
     !k v. FLOOKUP f1 k = SOME v ==>
           ?v2. FLOOKUP f2 k = SOME v2 /\ r v v2`;
@@ -112,7 +129,7 @@ val FMAP_REL_def = Define `
 (* state relation *)
 
 val state_rel_def = Define `
-  state_rel (s:'ffi closSem$state) (t:'ffi closSem$state) <=> 
+  state_rel (s:'ffi closSem$state) (t:'ffi closSem$state) <=>
     s.code = FEMPTY /\ t.code = FEMPTY /\
     t.max_app = s.max_app /\ 1 <= s.max_app /\
     t.clock = s.clock /\
@@ -123,20 +140,31 @@ val state_rel_def = Define `
 (* evaluation theorem *)
 
 val collect_args_IMP = store_thm("collect_args_IMP",
-  ``collect_args max_app k e1 = (num_args,e2) ==>
-    k <= num_args /\ num_args <= max_app``,
-  cheat);
+  ``!max_app k e1 num_args e2.
+      collect_args max_app k e1 = (num_args,e2) /\ k <= max_app ==>
+      k <= num_args /\ num_args <= max_app``,
+  recInduct collect_args_ind
+  \\ rpt conj_tac \\ rpt gen_tac \\ strip_tac
+  \\ fs [collect_args_def]
+  \\ rw [] \\ fs []);
 
 val collect_args_ok_IMP = store_thm("collect_args_ok_IMP",
-  ``collect_args max_app 1 e = (num_args,e2) /\ syntax_ok max_app [e] ==>
-    ?ts. e = mk_Fns ts e2 ∧ num_args = LENGTH ts /\ 
-         syntax_ok max_app [e2] /\ 0 < LENGTH ts``,
-  cheat);
-
-val HD_intro_multi = store_thm("HD_intro_multi",
-  ``[HD (intro_multi max_app [e2])] = intro_multi max_app [e2]``,
-  `?x. intro_multi max_app [e2] = [x]` by metis_tac [intro_multi_sing]
-  \\ fs []);
+  ``!max_app k e num_args e2.
+      collect_args max_app k e = (num_args,e2) /\ syntax_ok [e] ==>
+      ?ts. e = mk_Fns ts e2 ∧ num_args = k + LENGTH ts /\
+           syntax_ok [e2]``,
+  recInduct collect_args_ind
+  \\ rw [] \\ fs []
+  \\ fs [collect_args_def] \\ rveq
+  \\ TRY (fs [collect_args_def] \\ rveq
+          \\ qexists_tac `[]` \\ fs [mk_Fns_def] \\ NO_TAC)
+  \\ FULL_CASE_TAC \\ rveq
+  \\ TRY (fs [collect_args_def] \\ rveq
+          \\ qexists_tac `[]` \\ fs [mk_Fns_def] \\ NO_TAC)
+  \\ first_x_assum drule
+  \\ fs [syntax_ok_def] \\ rveq
+  \\ strip_tac \\ fs [] \\ rveq
+  \\ qexists_tac `t::ts` \\ fs [mk_Fns_def]);
 
 val dest_closure_SOME_IMP = store_thm("dest_closure_SOME_IMP",
   ``dest_closure max_app loc_opt f2 xs = SOME x ==>
@@ -154,25 +182,243 @@ val collect_apps_acc = prove(
   \\ IF_CASES_TAC \\ fs []
   \\ rw [] \\ res_tac \\ fs []);
 
-val collect_apps_prefix = prove(
-  ``collect_apps max_app xs e = (xs ++ ys, e2) ==>
-    collect_apps max_app [] e = (ys,e2)``,
-  cheat);
+val collect_apps_cons_lemma = prove(
+  ``!e1 m ys other e2.
+      collect_apps (m+LENGTH ys) ys e1 = (ys ++ other,e2) <=>
+      collect_apps m [] e1 = (other,e2)``,
+  Induct \\ fs [collect_apps_def]
+  \\ rw [] \\ Cases_on `o'` \\ fs [collect_apps_def]
+  \\ rw [] \\ fs []
+  \\ fs [LESS_EQ_EXISTS]
+  \\ Cases_on `collect_apps (p + LENGTH l) l e1`
+  \\ drule collect_apps_acc
+  \\ strip_tac \\ rveq \\ fs []
+  \\ Cases_on `collect_apps (p + (LENGTH l + LENGTH ys)) (ys ⧺ l) e1`
+  \\ drule collect_apps_acc
+  \\ strip_tac \\ rveq \\ fs []
+  \\ pop_assum mp_tac
+  \\ `(LENGTH l + LENGTH ys) = LENGTH (ys ++ l)` by fs []
+  \\ asm_rewrite_tac []
+  \\ rfs []);
 
 val collect_apps_cons = prove(
-  ``collect_apps max_app [x] e = (x::ys, e2) ==>
-    collect_apps max_app [] e = (ys,e2)``,
-  cheat);
+  ``!e1 m x other e2.
+      collect_apps m [x] e1 = (x::other,e2) /\ m <> 0 ==>
+      collect_apps (m-1) [] e1 = (other,e2)``,
+  once_rewrite_tac [collect_apps_cons_lemma |> GSYM
+       |> Q.SPECL [`e1`,`m`,`[x]`]
+       |> SIMP_RULE std_ss [LENGTH,APPEND]] \\ rw []);
 
-val collect_apps_err = prove(
-  ``evaluate (other,env1,s2') = (Rerr e'',s2) /\ 
-    collect_apps s2'.max_app [] e1 = (other,e2) ==>
-    evaluate ([e],env1,s2') = (Rerr e'',s2)``,
-  cheat);
+val mk_Apps_def = Define `
+  mk_Apps e [] = e /\
+  mk_Apps e ((t,other)::ts) = App t NONE (mk_Apps e ts) [other]`
+
+val collect_apps_IMP_mk_Apps = prove(
+  ``!es max_app (acc:closLang$exp list) e other e3.
+      collect_apps max_app [] e = (other,e3) /\ syntax_ok es /\ es = [e] ==>
+      ?ts. e = mk_Apps e3 (ZIP (ts, other)) /\ LENGTH other = LENGTH ts /\
+           LENGTH other <= max_app``,
+  recInduct (theorem "syntax_ok_ind") \\ fs [] \\ rw []
+  \\ fs [collect_apps_def] \\ rveq
+  \\ TRY (qexists_tac `[]` \\ fs [mk_Apps_def]
+          \\ FULL_CASE_TAC \\ fs [] \\ rveq \\ fs [mk_Apps_def] \\ NO_TAC)
+  \\ fs [syntax_ok_def] \\ rveq
+  \\ fs [collect_apps_def] \\ rveq
+  \\ FULL_CASE_TAC \\ fs [] \\ rveq
+  \\ TRY (qexists_tac `[]` \\ fs [mk_Apps_def] \\ NO_TAC)
+  \\ fs [syntax_ok_def]
+  \\ Cases_on `es` \\ fs [] \\ rveq
+  \\ imp_res_tac collect_apps_acc \\ rveq \\ fs []
+  \\ drule (GEN_ALL collect_apps_cons) \\ fs []
+  \\ strip_tac \\ first_x_assum drule
+  \\ strip_tac \\ rveq \\ fs []
+  \\ qexists_tac `t::ts` \\ fs [ZIP,mk_Apps_def])
+  |> SIMP_RULE std_ss [];
+
+val mk_Apps_err_1 = prove(
+  ``∀ts other env1 s1 e3.
+      evaluate (other,env1,s1) = (Rerr e2,s2) /\
+      LENGTH other = LENGTH ts ==>
+      evaluate ([mk_Apps e3 (ZIP (ts,other))],env1,s1) = (Rerr e2,s2)``,
+  Induct
+  \\ fs [evaluate_def]
+  \\ Cases_on `other` \\ fs [ZIP,mk_Apps_def]
+  \\ once_rewrite_tac [evaluate_CONS]
+  \\ rw [] \\ fs [case_eq_thms,pair_case_eq]
+  \\ rveq \\ fs [] \\ fs [evaluate_def]);
+
+val mk_Apps_err_2 = prove(
+  ``∀ts other env1 s1 e3 vs.
+      evaluate ([e3],env1,s2) = (Rerr e2,s2') /\
+      evaluate (other,env1,s1) = (Rval vs,s2) /\
+      LENGTH other = LENGTH ts ==>
+      evaluate ([mk_Apps e3 (ZIP (ts,other))],env1,s1) = (Rerr e2,s2')``,
+  Induct
+  \\ fs [evaluate_def,mk_Apps_def]
+  \\ Cases_on `other` \\ fs [ZIP,mk_Apps_def]
+  \\ once_rewrite_tac [evaluate_CONS]
+  \\ rw [] \\ fs [case_eq_thms,pair_case_eq]
+  \\ rveq \\ fs [] \\ fs [evaluate_def]
+  \\ imp_res_tac evaluate_SING \\ rveq \\ fs []);
+
+val collect_apps_syntax_ok = store_thm("collect_apps_syntax_ok",
+  ``!k aux e res e1.
+      collect_apps k aux e = (res,e1) /\
+      syntax_ok [e] /\ syntax_ok aux ==>
+      syntax_ok res /\ syntax_ok [e1]``,
+  recInduct collect_apps_ind
+  \\ rw [collect_apps_def] \\ fs []
+  \\ fs [syntax_ok_def]);
+
+val evaluate_mk_Apps_err = prove(
+  ``!other ts env1 s1 vs.
+      evaluate (other,env1,s1) = (Rval vs,s3) /\
+      evaluate ([e],env1,s3) = (Rerr e3,s2') /\
+      LENGTH other = LENGTH ts ==>
+      evaluate ([mk_Apps e (ZIP (ts,other))],env1,s1) = (Rerr e3,s2')``,
+  Induct \\ Cases_on `ts` \\ fs [mk_Apps_def]
+  \\ fs [evaluate_def]
+  \\ simp [Once evaluate_CONS] \\ rw []
+  \\ fs [case_eq_thms,pair_case_eq] \\ rveq);
+
+val evaluate_apps_def = Define `
+  evaluate_apps f [] s = (Rval [f], s) /\
+  evaluate_apps f (x::xs) s =
+    case evaluate_apps f xs s of
+    | (Rval [v], s1) => evaluate_app NONE v [x] s1
+    | res => res`;
+
+val evaluate_mk_Apps_ok = prove(
+  ``!other ts env1 s1 vs.
+      evaluate ([e],env1,s3) = (Rval [f],s2') /\
+      evaluate (other,env1,s1) = (Rval vs,s3) /\
+      LENGTH other = LENGTH ts ==>
+      evaluate ([mk_Apps e (ZIP (ts,other))],env1,s1) =
+      evaluate_apps f vs s2'``,
+  once_rewrite_tac [CONJ_COMM]
+  \\ Induct \\ Cases_on `ts` \\ fs [mk_Apps_def]
+  \\ fs [evaluate_def,evaluate_apps_def]
+  \\ simp [Once evaluate_CONS] \\ rw []
+  \\ fs [case_eq_thms,pair_case_eq] \\ rveq
+  \\ first_x_assum (qspec_then `t` mp_tac) \\ fs []
+  \\ rpt (disch_then drule)
+  \\ strip_tac \\ fs []
+  \\ Cases_on `evaluate_apps f vs' s2'` \\ fs []
+  \\ imp_res_tac evaluate_SING \\ fs []
+  \\ rveq \\ fs []
+  \\ fs [evaluate_apps_def]
+  \\ Cases_on `q` \\ fs []
+  \\ imp_res_tac evaluate_SING \\ fs []
+  \\ rveq \\ fs []);
+
+val dest_closure_NONE_IMP_apps = prove(
+  ``!xs f1 s1.
+      dest_closure s1.max_app NONE f1 [LAST xs] = NONE /\ xs <> [] ==>
+      evaluate_apps f1 xs s1 = (Rerr (Rabort Rtype_error),s1)``,
+  Induct \\ fs [evaluate_apps_def]
+  \\ Cases_on `xs` \\ fs [evaluate_apps_def]
+  \\ fs [evaluate_apps_def,evaluate_def]);
+
+val evaluate_apps_SNOC = prove(
+  ``!xs x f s.
+      evaluate_apps f (SNOC x xs) s =
+      case evaluate_app NONE f [x] s of
+      | (Rval [v], s) => evaluate_apps v xs s
+      | res => res``,
+  Induct
+  THEN1 (fs [evaluate_apps_def] \\ rw []
+         \\ every_case_tac \\ fs [])
+  \\ fs [SNOC_APPEND]
+  \\ fs [evaluate_apps_def] \\ rw []
+  \\ Cases_on `evaluate_app NONE f [x] s` \\ fs []
+  \\ Cases_on `q` \\ fs []
+  \\ Cases_on `a` \\ fs []
+  \\ Cases_on `t` \\ fs []);
+
+val evaluate_apps_Clos_timeout = prove(
+  ``!ys ts s1 e1 env.
+      s1.clock < LENGTH ys /\ LENGTH ys <= LENGTH ts /\
+      1 ≤ s1.max_app ==>
+      evaluate_apps (Closure NONE [] env 1 (mk_Fns ts e1))
+        ys s1 = (Rerr (Rabort Rtimeout_error),s1 with clock := 0)``,
+  recInduct SNOC_INDUCT \\ rw []
+  \\ fs [evaluate_apps_SNOC]
+  \\ fs [evaluate_def,dest_closure_def,check_loc_def]
+  \\ IF_CASES_TAC \\ fs []
+  \\ Cases_on `ts` \\ fs [mk_Fns_def,evaluate_def]
+  \\ fs [EVAL ``(dec_clock 1 s).max_app``]
+  \\ `(dec_clock 1 s1).clock < LENGTH l` by (EVAL_TAC \\ fs [])
+  \\ first_x_assum drule
+  \\ fs [dec_clock_def]);
+
+val evaluate_apps_Clos_timeout_alt = prove(
+  ``!ys ts s1 e1 env.
+      s1.clock <= LENGTH ts /\ LENGTH ts < LENGTH ys /\
+      1 ≤ s1.max_app ==>
+      evaluate_apps (Closure NONE [] env 1 (mk_Fns ts e1))
+        ys s1 = (Rerr (Rabort Rtimeout_error),s1 with clock := 0)``,
+  recInduct SNOC_INDUCT \\ rw []
+  \\ fs [evaluate_apps_SNOC]
+  \\ fs [evaluate_def,dest_closure_def,check_loc_def]
+  \\ IF_CASES_TAC \\ fs []
+  \\ Cases_on `ts` \\ fs [mk_Fns_def,evaluate_def]
+  \\ fs [EVAL ``(dec_clock 1 s).max_app``]
+  \\ `(dec_clock 1 s1).clock <= LENGTH t` by (EVAL_TAC \\ fs [])
+  \\ first_x_assum drule
+  \\ fs [dec_clock_def]);
+
+val evaluate_apps_Clos_short = prove(
+  ``!ys ts s1 e1 env.
+      LENGTH ys <= s1.clock /\ LENGTH ys <= LENGTH ts /\
+      1 ≤ s1.max_app ==>
+      evaluate_apps (Closure NONE [] env 1 (mk_Fns ts e1)) ys s1 =
+         (Rval [Closure NONE [] (ys ++ env) 1
+                   (mk_Fns (DROP (LENGTH ys) ts) e1)],
+          dec_clock (LENGTH ys) s1)``,
+  recInduct SNOC_INDUCT \\ rw []
+  \\ fs [evaluate_apps_SNOC,evaluate_apps_def]
+  THEN1 (fs [state_component_equality,dec_clock_def])
+  \\ fs [evaluate_def,dest_closure_def,check_loc_def]
+  \\ Cases_on `ts` \\ fs [mk_Fns_def,evaluate_def]
+  \\ fs [EVAL ``(dec_clock 1 s).max_app``]
+  \\ `LENGTH l <= (dec_clock 1 s1).clock` by (EVAL_TAC \\ fs [])
+  \\ first_x_assum drule
+  \\ fs [EVAL ``(dec_clock 1 s).max_app``]
+  \\ disch_then drule
+  \\ fs [dec_clock_def,ADD1]);
+
+val evaluate_apps_Clos_long = prove(
+  ``!ys ts s1 e1 env.
+      LENGTH ts < s1.clock /\ LENGTH ts < LENGTH ys /\
+      1 ≤ s1.max_app ==>
+      evaluate_apps (Closure NONE [] env 1 (mk_Fns ts e1)) ys s1 =
+        case evaluate ([e1],REVERSE (TAKE (1+LENGTH ts) (REVERSE ys)) ++ env,
+                dec_clock (1+LENGTH ts) s1) of
+        | (Rval [v],s) =>
+             evaluate_apps v (REVERSE (DROP (1+LENGTH ts) (REVERSE ys))) s
+        | res => res``,
+  recInduct SNOC_INDUCT \\ rw []
+  \\ fs [evaluate_apps_SNOC,evaluate_apps_def]
+  \\ fs [evaluate_def,Once dest_closure_def,check_loc_def]
+  \\ Cases_on `ts` \\ fs [mk_Fns_def,evaluate_def]
+  THEN1
+   (fs [REVERSE_SNOC]
+    \\ Cases_on `evaluate ([e1],x::env,dec_clock 1 s1)` \\ fs []
+    \\ Cases_on `q` \\ fs []
+    \\ Cases_on `a` \\ fs []
+    \\ Cases_on `t` \\ fs [])
+  \\ fs [EVAL ``(dec_clock 1 s).max_app``]
+  \\ `LENGTH t < (dec_clock 1 s1).clock` by (EVAL_TAC \\ fs [])
+  \\ first_x_assum drule
+  \\ fs [EVAL ``(dec_clock 1 s).max_app``]
+  \\ disch_then kall_tac
+  \\ fs [REVERSE_SNOC] \\ fs [ADD1]
+  \\ fs [dec_clock_def,ADD1]
+  \\ simp_tac std_ss [GSYM APPEND_ASSOC,APPEND]);
 
 val evaluate_intro_multi = Q.store_thm("evaluate_intro_multi",
   `(!ys env2 (t1:'ffi closSem$state) env1 t2 s1 res2 xs.
-     (evaluate (ys,env2,t1) = (res2,t2)) /\ 
+     (evaluate (ys,env2,t1) = (res2,t2)) /\
      EVERY2 (v_rel s1.max_app) env1 env2 /\
      state_rel s1 t1 /\ code_rel s1.max_app xs ys ==>
      ?res1 s2.
@@ -182,101 +428,190 @@ val evaluate_intro_multi = Q.store_thm("evaluate_intro_multi",
    (!loc_opt f2 args2 (t1:'ffi closSem$state) res2 t2 f1 args1 s1.
      (evaluate_app loc_opt f2 args2 t1 = (res2,t2)) /\ loc_opt = NONE /\
      v_rel s1.max_app f1 f2 /\ EVERY2 (v_rel s1.max_app) args1 args2 /\
-     state_rel s1 t1 ==>
+     state_rel s1 t1 /\ LENGTH args1 <= s1.max_app ==>
      ?res1 s2.
-       (evaluate_app loc_opt f1 args1 s1 = (res1,s2)) /\
-       result_rel (LIST_REL (v_rel s1.max_app)) (v_rel s1.max_app) res1 res2 /\ 
+       (evaluate_apps f1 args1 s1 = (res1,s2)) /\
+       result_rel (LIST_REL (v_rel s1.max_app)) (v_rel s1.max_app) res1 res2 /\
        state_rel s2 t2)`,
-
-  HO_MATCH_MP_TAC (evaluate_ind |> Q.SPEC `λ(x1,x2,x3). P0 x1 x2 x3` 
+  HO_MATCH_MP_TAC (evaluate_ind |> Q.SPEC `λ(x1,x2,x3). P0 x1 x2 x3`
                    |> Q.GEN `P0` |> SIMP_RULE std_ss [FORALL_PROD])
   \\ rpt strip_tac
   \\ TRY (drule code_rel_IMP_LENGTH \\ strip_tac)
   THEN1 (* NIL *)
    (fs [evaluate_def] \\ rveq \\ fs [])
-  THEN1 (* CONS *) 
+  THEN1 (* CONS *)
    (rename1 `_ = LENGTH zs`
     \\ Cases_on `zs` THEN1 fs [LENGTH]
     \\ Cases_on `t` THEN1 fs [LENGTH]
     \\ fs [evaluate_def,closSemTheory.case_eq_thms,pair_case_eq]
     \\ rveq \\ fs []
     \\ first_x_assum drule \\ fs [code_rel_CONS_CONS]
-    \\ disch_then drule \\ strip_tac \\ fs []     
-    \\ Cases_on `res1` \\ fs []     
+    \\ disch_then drule \\ strip_tac \\ fs []
+    \\ Cases_on `res1` \\ fs []
     \\ `s1.max_app = s2'.max_app` by (imp_res_tac evaluate_const \\ fs [])
     \\ fs [] \\ first_x_assum drule \\ fs []
-    \\ disch_then drule \\ strip_tac \\ fs []     
-    \\ Cases_on `res1` \\ fs []     
+    \\ disch_then drule \\ strip_tac \\ fs []
+    \\ Cases_on `res1` \\ fs []
     \\ imp_res_tac evaluate_SING \\ rveq \\ fs [])
-  THEN1
+  THEN1 (* Var *)
    (Cases_on `xs` \\ fs [] \\ rveq
     \\ Cases_on `h` \\ fs [code_rel_def,intro_multi_def] \\ rveq \\ fs []
     \\ fs [syntax_ok_def] \\ rveq \\ fs [intro_multi_def]
+    \\ TRY pairarg_tac \\ fs []
     \\ fs [evaluate_def]
     \\ imp_res_tac LIST_REL_LENGTH \\ fs []
     \\ IF_CASES_TAC \\ fs [] \\ rveq \\ fs []
-    \\ fs [LIST_REL_EL_EQN]) 
-  THEN1 (* If *) cheat
-  THEN1 (* Let *) cheat
-  THEN1 (* Raise *) cheat
-  THEN1 (* Handle *) cheat
-  THEN1 (* Op *) cheat
-  THEN1 (* Fn *) 
+    \\ fs [LIST_REL_EL_EQN])
+  THEN1 (* If *)
    (Cases_on `xs` \\ fs [] \\ rveq
     \\ Cases_on `h` \\ fs [code_rel_def,intro_multi_def] \\ rveq \\ fs []
     \\ fs [syntax_ok_def] \\ rveq \\ fs [intro_multi_def]
-    \\ pairarg_tac \\ fs [] \\ rveq
+    \\ TRY pairarg_tac \\ fs []
+    \\ reverse (fs [evaluate_def,case_eq_thms,pair_case_eq] \\ rveq)
+    \\ fs [HD_intro_multi]
+    THEN1
+     (first_x_assum drule \\ fs []
+      \\ disch_then (qspec_then `[e]` mp_tac) \\ fs []
+      \\ strip_tac \\ fs [])
+    \\ first_x_assum drule \\ fs []
+    \\ disch_then (qspec_then `[e]` mp_tac) \\ fs []
+    \\ strip_tac \\ fs []
+    \\ Cases_on `res1` \\ fs []
+    \\ imp_res_tac evaluate_SING \\ fs []
+    \\ rveq \\ fs []
+    \\ `(Boolv T = y <=> Boolv T = r1) /\
+        (Boolv F = y <=> Boolv F = r1)` by
+     (fs [EVAL ``closSem$Boolv T``,EVAL ``closSem$Boolv F``]
+      \\ qpat_x_assum `v_rel _ _ _` mp_tac
+      \\ rpt (pop_assum kall_tac)
+      \\ rw [] \\ eq_tac \\ rw []
+      \\ rpt (pop_assum mp_tac)
+      \\ simp [Once v_rel_cases])
+    \\ ntac 2 (pop_assum (fn th => fs [th]))
+    \\ IF_CASES_TAC \\ fs [] \\ rveq
+    \\ `s1.max_app = s2.max_app` by (imp_res_tac evaluate_const \\ fs [])
+    \\ fs [] \\ IF_CASES_TAC \\ fs [] \\ rveq \\ fs[])
+  THEN1 (* Let *)
+   (Cases_on `xs` \\ fs [] \\ rveq
+    \\ Cases_on `h` \\ fs [code_rel_def,intro_multi_def] \\ rveq \\ fs []
+    \\ fs [syntax_ok_def] \\ rveq \\ fs [intro_multi_def]
+    \\ TRY pairarg_tac \\ fs [evaluate_def,HD_intro_multi]
+    \\ reverse (fs [evaluate_def,case_eq_thms,pair_case_eq] \\ rveq)
+    \\ first_x_assum drule \\ fs []
+    \\ disch_then drule \\ fs []
+    \\ disch_then (qspec_then `l` mp_tac) \\ fs []
+    \\ strip_tac \\ fs []
+    \\ Cases_on `res1` \\ fs []
+    \\ `s1.max_app = s2.max_app` by (imp_res_tac evaluate_const \\ fs [])
+    \\ fs [] \\ first_x_assum match_mp_tac
+    \\ fs [] \\ metis_tac [EVERY2_APPEND])
+  THEN1 (* Raise *)
+   (Cases_on `xs` \\ fs [] \\ rveq
+    \\ Cases_on `h` \\ fs [code_rel_def,intro_multi_def] \\ rveq \\ fs []
+    \\ fs [syntax_ok_def] \\ rveq \\ fs [intro_multi_def]
+    \\ TRY pairarg_tac \\ fs []
+    \\ fs [evaluate_def,case_eq_thms,pair_case_eq] \\ rveq
+    \\ fs [HD_intro_multi]
+    \\ first_x_assum drule \\ fs []
+    \\ disch_then (qspec_then `[e]` mp_tac) \\ fs []
+    \\ strip_tac \\ fs []
+    \\ Cases_on `res1` \\ fs []
+    \\ imp_res_tac evaluate_SING \\ fs [] \\ rw [])
+  THEN1 (* Handle *)
+   (Cases_on `xs` \\ fs [] \\ rveq
+    \\ Cases_on `h` \\ fs [code_rel_def,intro_multi_def] \\ rveq \\ fs []
+    \\ fs [syntax_ok_def] \\ rveq \\ fs [intro_multi_def]
+    \\ TRY pairarg_tac \\ fs [evaluate_def,HD_intro_multi]
+    \\ reverse (fs [evaluate_def,case_eq_thms,pair_case_eq] \\ rveq)
+    \\ first_x_assum drule \\ fs []
+    \\ disch_then drule \\ fs []
+    \\ disch_then (qspec_then `[e]` mp_tac) \\ fs []
+    \\ strip_tac \\ fs [PULL_EXISTS]
+    \\ Cases_on `res1` \\ fs [] \\ rveq \\ fs[]
+    \\ `s1.max_app = s2.max_app` by (imp_res_tac evaluate_const \\ fs [])
+    \\ fs [] \\ first_x_assum match_mp_tac)
+  THEN1 (* Op *) cheat
+  THEN1 (* Fn *)
+   (Cases_on `xs` \\ fs [] \\ rveq
+    \\ Cases_on `h` \\ fs [code_rel_def,intro_multi_def] \\ rveq \\ fs []
+    \\ fs [syntax_ok_def] \\ rveq \\ fs [intro_multi_def]
+    \\ TRY pairarg_tac \\ fs [] \\ rveq
     \\ `1 <= s1.max_app` by fs [state_rel_def]
     \\ fs [evaluate_def]
-    \\ imp_res_tac collect_args_IMP \\ fs []
+    \\ drule (GEN_ALL collect_args_IMP) \\ fs [] \\ strip_tac
     \\ `t1.max_app = s1.max_app` by fs [state_rel_def] \\ fs []
     \\ rveq \\ fs []
     \\ once_rewrite_tac [v_rel_cases] \\ fs [code_rel_def]
     \\ rename1 `_ = (_,e2)` \\ qexists_tac `e2`
     \\ fs [HD_intro_multi]
-    \\ match_mp_tac collect_args_ok_IMP \\ fs [])    
-  THEN1 (* Letrec *) 
+    \\ drule collect_args_ok_IMP \\ fs [])
+  THEN1 (* Letrec *)
    (Cases_on `xs` \\ fs [] \\ rveq
     \\ Cases_on `h` \\ fs [code_rel_def,intro_multi_def] \\ rveq \\ fs []
     \\ fs [syntax_ok_def] \\ rveq \\ fs [intro_multi_def]
     \\ TRY pairarg_tac \\ fs [] \\ rveq \\ fs [])
-
-  THEN1 (* App *) 
+  THEN1 (* App *)
    (Cases_on `xs` \\ fs [] \\ rveq
     \\ Cases_on `h` \\ fs [code_rel_def,intro_multi_def] \\ rveq \\ fs []
     \\ fs [syntax_ok_def] \\ rveq \\ fs [intro_multi_def]
     \\ TRY pairarg_tac \\ fs [] \\ rveq \\ fs []
     \\ fs [intro_multi_length]
     \\ fs [DECIDE ``n > 0n <=> n <> 0``]
-    \\ imp_res_tac collect_apps_acc \\ rveq 
+    \\ imp_res_tac collect_apps_acc \\ rveq
     \\ `?x. l = [x]` by (Cases_on `l` \\ fs [] \\ Cases_on `t`) \\ rveq \\ fs []
-    \\ `syntax_ok s1.max_app other /\ 
-        syntax_ok s1.max_app (x::other)` by cheat
+    \\ `syntax_ok other /\ syntax_ok (x::other) /\ syntax_ok [e']` by
+     (drule collect_apps_syntax_ok \\ fs []
+      \\ once_rewrite_tac [syntax_ok_cons] \\ fs [])
+    \\ drule collect_apps_cons
+    \\ impl_tac THEN1 fs [state_rel_def] \\ strip_tac
+    \\ drule collect_apps_IMP_mk_Apps \\ fs []
+    \\ strip_tac \\ rveq \\ fs [GSYM mk_Apps_def]
     \\ fs [evaluate_def]
     \\ fs [intro_multi_length]
     \\ fs [DECIDE ``n > 0n <=> n <> 0``]
     \\ reverse (fs [closSemTheory.case_eq_thms,pair_case_eq])
     \\ rveq \\ fs []
     \\ first_x_assum drule \\ fs []
-    \\ disch_then (qspec_then `x::other` mp_tac) \\ fs [] 
+    \\ disch_then (qspec_then `x::other` mp_tac) \\ fs []
     \\ strip_tac \\ Cases_on `res1` \\ fs [] \\ rveq
+    \\ rewrite_tac [GSYM ZIP]
     THEN1
-     (qpat_x_assum `evaluate (x::other,env1,s1) = _` mp_tac
-      \\ simp [Once evaluate_CONS]
-      \\ fs [closSemTheory.case_eq_thms,pair_case_eq]
-      \\ reverse strip_tac \\ rveq \\ fs [] \\ rveq \\ fs []
-      \\ imp_res_tac collect_apps_cons
-      \\ `s1.max_app = s2'.max_app` by (imp_res_tac evaluate_const \\ fs [])
-      \\ fs [] \\ imp_res_tac collect_apps_err \\ fs [])            
-    \\ cheat)
-
-  THEN1 (* Tick *) 
+     (drule (GEN_ALL mk_Apps_err_1)
+      \\ disch_then (qspec_then `t::ts` mp_tac) \\ fs [])
+    THEN1
+     (rename1 `_ = (Rval vs, s3)`
+      \\ first_x_assum (qspecl_then [`env1`,`s3`,`[e']`] mp_tac)
+      \\ impl_tac THEN1 (imp_res_tac evaluate_const \\ fs [])
+      \\ strip_tac \\ rveq
+      \\ drule (GEN_ALL mk_Apps_err_2)
+      \\ disch_then (qspec_then `t::ts` mp_tac) \\ fs []
+      \\ disch_then drule
+      \\ fs [] \\ imp_res_tac evaluate_const \\ fs [])
+    \\ rename1 `_ = (Rval vs, s3)`
+    \\ first_x_assum (qspecl_then [`env1`,`s3`,`[e']`] mp_tac)
+    \\ impl_tac THEN1 (imp_res_tac evaluate_const \\ fs [])
+    \\ strip_tac \\ rveq
+    \\ Cases_on `res1` \\ fs []
+    \\ drule evaluate_SING \\ strip_tac \\ rveq
+    \\ drule (GEN_ALL evaluate_mk_Apps_ok)
+    \\ disch_then drule
+    \\ disch_then (qspec_then `t::ts` assume_tac) \\ rfs []
+    \\ rveq \\ fs []
+    \\ `s1.max_app = s2'.max_app` by (imp_res_tac evaluate_const \\ fs [])
+    \\ `s3.max_app = s2'.max_app` by (imp_res_tac evaluate_const \\ fs [])
+    \\ fs [GSYM CONJ_ASSOC]
+    \\ first_x_assum drule
+    \\ rpt (disch_then drule)
+    \\ impl_tac \\ fs []
+    \\ imp_res_tac evaluate_IMP_LENGTH \\ fs [intro_multi_length]
+    \\ fs [state_rel_def])
+  THEN1 (* Tick *)
    (`t1.clock = s1.clock` by fs [state_rel_def]
     \\ Cases_on `xs` \\ fs [] \\ rveq
     \\ Cases_on `h` \\ fs [code_rel_def,intro_multi_def] \\ rveq \\ fs []
     \\ fs [syntax_ok_def] \\ rveq \\ fs [intro_multi_def]
     \\ TRY pairarg_tac \\ fs []
-    \\ fs [evaluate_def,case_eq_thms] 
+    \\ fs [evaluate_def,case_eq_thms]
     \\ IF_CASES_TAC \\ fs [] \\ rveq \\ fs []
     \\ `LIST_REL (v_rel (dec_clock 1 s1).max_app) env1 env2` by fs [dec_clock_def]
     \\ first_x_assum drule
@@ -285,44 +620,141 @@ val evaluate_intro_multi = Q.store_thm("evaluate_intro_multi",
     \\ fs [HD_intro_multi]
     \\ impl_tac \\ fs []
     \\ fs [state_rel_def])
-  THEN1 (* Call *) 
+  THEN1 (* Call *)
    (Cases_on `xs` \\ fs [] \\ rveq
     \\ Cases_on `h` \\ fs [code_rel_def,intro_multi_def] \\ rveq \\ fs []
     \\ fs [syntax_ok_def] \\ rveq \\ fs [intro_multi_def]
     \\ TRY pairarg_tac \\ fs [])
-  THEN1 (* app NIL *) 
-   (fs [evaluate_def] \\ rveq \\ fs [])
-  (* app CONS *) 
+  THEN1 (* app NIL *)
+   (fs [evaluate_def,evaluate_apps_def] \\ rveq \\ fs [])
+  (* app CONS *)
   \\ fs [evaluate_def] \\ rveq \\ fs []
   \\ fs [case_eq_thms] \\ fs [] \\ rveq
-  THEN1 (* dest_closure returns NONE *) 
-   (qsuff_tac `dest_closure s1.max_app NONE f1 (x::xs) = NONE` THEN1 fs []
-    \\ fs [dest_closure_def,case_eq_thms]
-    \\ qpat_x_assum `v_rel _ f1 f2` mp_tac 
-    \\ once_rewrite_tac [v_rel_cases] \\ fs []    
-    \\ strip_tac \\ fs [] \\ rveq \\ fs [check_loc_def]
-    \\ imp_res_tac LIST_REL_LENGTH \\ fs [state_rel_def]
-    \\ CCONTR_TAC \\ fs []
-    \\ every_case_tac \\ fs [])
-  
-  THEN1 (* dest_closure returns Patrial_app *) 
-   (qpat_x_assum `v_rel _ f1 f2` mp_tac 
-    \\ once_rewrite_tac [v_rel_cases] \\ fs []    
+  THEN1 (* dest_closure returns NONE *)
+   (`?y. dest_closure s1.max_app NONE f1 (x::xs) = NONE` by
+     (fs [dest_closure_def,case_eq_thms]
+      \\ qpat_x_assum `v_rel _ f1 f2` mp_tac
+      \\ once_rewrite_tac [v_rel_cases] \\ fs []
+      \\ strip_tac \\ fs [] \\ rveq \\ fs [check_loc_def]
+      \\ imp_res_tac LIST_REL_LENGTH \\ fs [state_rel_def]
+      \\ CCONTR_TAC \\ fs []
+      \\ every_case_tac \\ fs [])
+    \\ `dest_closure s1.max_app NONE f1 [LAST (x::xs)] = NONE` by
+     (pop_assum mp_tac
+      \\ simp [dest_closure_def,case_eq_thms,UNCURRY] \\ rw []
+      \\ qpat_x_assum `v_rel _ f1 f2` mp_tac
+      \\ once_rewrite_tac [v_rel_cases] \\ fs []
+      \\ strip_tac \\ fs [] \\ rveq \\ fs [check_loc_def])
+    \\ drule dest_closure_NONE_IMP_apps \\ fs [])
+  THEN1 (* dest_closure returns Patrial_app *)
+   (qpat_x_assum `v_rel _ f1 f2` mp_tac
+    \\ once_rewrite_tac [v_rel_cases] \\ fs []
     \\ drule dest_closure_SOME_IMP \\ strip_tac \\ fs []
     \\ strip_tac \\ fs [] \\ rveq
     (* needs case for Recclosure *)
-    \\ qpat_x_assum `_ = SOME (Partial_app _)` mp_tac   
-    \\ simp [Once dest_closure_def] 
+    \\ qpat_x_assum `_ = SOME (Partial_app _)` mp_tac
+    \\ simp [Once dest_closure_def]
     \\ IF_CASES_TAC \\ fs [] \\ strip_tac \\ rveq \\ fs []
-    \\ fs [dest_closure_def,check_loc_def]
-    \\ `s1.clock = t1.clock` by fs [state_rel_def] 
-    \\ Cases_on `s1.clock = 0` \\ fs []
-    THEN1 (imp_res_tac LIST_REL_LENGTH \\ rveq \\ fs [state_rel_def])
-    \\ cheat)  
-  (* dest_closure returns Full_app *) 
-  \\ cheat);
+    \\ fs [dest_closure_def,check_loc_def,ADD1]
+    \\ `s1.clock = t1.clock` by fs [state_rel_def] \\ fs []
+    \\ imp_res_tac (GSYM LIST_REL_LENGTH) \\ fs []
+    \\ `LENGTH xs < LENGTH ts` by fs []
+    \\ Cases_on `t1.clock < LENGTH xs + 1` \\ fs [] \\ rveq \\ fs []
+    THEN1
+     (qexists_tac `s1 with clock := 0`
+      \\ reverse conj_tac THEN1 fs [state_rel_def]
+      \\ match_mp_tac (GEN_ALL evaluate_apps_Clos_timeout) \\ fs [])
+    \\ fs [evaluate_apps_Clos_short,ADD1]
+    \\ reverse conj_tac THEN1 fs [state_rel_def,ADD1,dec_clock_def]
+    \\ simp [Once v_rel_cases]
+    \\ qexists_tac `x::xs ++ args1`
+    \\ qexists_tac `env1` \\ fs []
+    \\ qexists_tac `e1` \\ fs []
+    \\ qexists_tac `(DROP (LENGTH xs + 1) ts)` \\ fs []
+    \\ imp_res_tac LIST_REL_LENGTH
+    \\ imp_res_tac LIST_REL_APPEND_EQ \\ fs [])
+  (* dest_closure returns Full_app *)
+  \\ Cases_on `t1.clock < SUC (LENGTH v69) − LENGTH rest_args` \\ fs []
+  THEN1
+   (qpat_x_assum `v_rel _ f1 f2` mp_tac
+    \\ once_rewrite_tac [v_rel_cases] \\ fs []
+    \\ drule dest_closure_SOME_IMP \\ strip_tac \\ fs []
+    \\ strip_tac \\ fs [] \\ rveq
+    \\ qpat_x_assum `_ = SOME _` mp_tac
+    \\ simp [Once dest_closure_def]
+    \\ IF_CASES_TAC \\ fs [] \\ strip_tac \\ rveq \\ fs [NOT_LESS]
+    \\ qexists_tac `s1 with clock := 0`
+    \\ reverse conj_tac THEN1 fs [state_rel_def]
+    \\ match_mp_tac evaluate_apps_Clos_timeout_alt
+    \\ fs [check_loc_def,state_rel_def]
+    \\ imp_res_tac LIST_REL_LENGTH \\ fs [ADD1])
+  \\ qpat_x_assum `v_rel _ f1 f2` mp_tac
+  \\ once_rewrite_tac [v_rel_cases] \\ fs []
+  \\ drule dest_closure_SOME_IMP \\ strip_tac \\ fs []
+  \\ strip_tac \\ fs [] \\ rveq
+  \\ qpat_x_assum `_ = SOME _` mp_tac
+  \\ simp [Once dest_closure_def,check_loc_def,ADD1]
+  \\ qmatch_goalsub_abbrev_tac `Full_app e e5 e6`
+  \\ IF_CASES_TAC \\ fs [] \\ strip_tac \\ rveq \\ fs [NOT_LESS]
+  \\ imp_res_tac (GSYM LIST_REL_LENGTH) \\ fs []
+  \\ `LENGTH e6 = LENGTH xs - LENGTH ts` by simp [Abbr `e6`] \\ fs []
+  \\ `LENGTH ts < s1.clock` by fs [state_rel_def]
+  \\ `LENGTH ts < LENGTH (x::xs)` by fs []
+  \\ drule evaluate_apps_Clos_long \\ simp []
+  \\ disch_then drule \\ fs []
+  \\ disch_then kall_tac \\ fs [ADD1]
+  \\ qmatch_goalsub_abbrev_tac `([_],e7,_)`
+  \\ Cases_on `evaluate ([e],e5,dec_clock (LENGTH ts + 1) t1)` \\ fs []
+  \\ `LIST_REL (v_rel (dec_clock (LENGTH ts + 1) s1).max_app) e7 e5` by
+   (unabbrev_all_tac
+    \\ match_mp_tac EVERY2_APPEND_suff \\ fs [dec_clock_def]
+    \\ match_mp_tac EVERY2_APPEND_suff \\ fs [dec_clock_def]
+    \\ match_mp_tac EVERY2_REVERSE
+    \\ match_mp_tac EVERY2_TAKE
+    \\ match_mp_tac EVERY2_APPEND_suff \\ fs [dec_clock_def]
+    \\ match_mp_tac EVERY2_REVERSE \\ fs [])
+  \\ first_x_assum drule
+  \\ disch_then (qspec_then `[e1]` mp_tac)
+  \\ fs [EVAL ``(dec_clock n s).max_app``]
+  \\ impl_tac THEN1 fs [state_rel_def,dec_clock_def]
+  \\ strip_tac \\ fs []
+  \\ Cases_on `q` \\ fs [] \\ rveq \\ fs []
+  \\ Cases_on `res1` \\ fs []
+  \\ Cases_on `a` \\ fs [] \\ rveq
+  \\ Cases_on `t` \\ fs [] \\ rveq \\ fs []
+  \\ qmatch_goalsub_abbrev_tac `evaluate_apps _ e8`
+  \\ rename1 `v_rel s1.max_app f1 f2`
+  \\ `v_rel s2.max_app f1 f2` by
+      (imp_res_tac evaluate_const \\ fs [dec_clock_def])
+  \\ first_x_assum drule
+  \\ `LIST_REL (v_rel s2.max_app) e8 e6` by
+   (unabbrev_all_tac
+    \\ match_mp_tac EVERY2_REVERSE
+    \\ match_mp_tac EVERY2_DROP
+    \\ match_mp_tac EVERY2_APPEND_suff \\ fs []
+    \\ imp_res_tac evaluate_const \\ fs [dec_clock_def]
+    \\ match_mp_tac EVERY2_REVERSE \\ fs [])
+  \\ rpt (disch_then drule)
+  \\ impl_tac THEN1
+   (unabbrev_all_tac \\ fs []
+    \\ imp_res_tac evaluate_const \\ fs [dec_clock_def])
+  \\ strip_tac \\ fs []
+  \\ imp_res_tac evaluate_const
+  \\ fs [dec_clock_def]);
 
-      
+val intro_multi_correct = store_thm("intro_multi_correct",
+  ``!xs env1 s1 res1 s2 env2 t2 t1.
+      evaluate (xs,env1,s1) = (res1,s2) /\ syntax_ok xs /\
+      LIST_REL (v_rel s1.max_app) env1 env2 /\ state_rel s1 t1 ==>
+      ?res2 t2.
+        evaluate (intro_multi s1.max_app xs,env2,t1) = (res2,t2) /\
+        result_rel (LIST_REL (v_rel s1.max_app)) (v_rel s1.max_app) res1
+          res2 /\ state_rel s2 t2``,
+  rpt gen_tac
+  \\ Cases_on `evaluate (intro_multi s1.max_app xs,env2,t1)` \\ fs []
+  \\ drule (CONJUNCT1 evaluate_intro_multi)
+  \\ ntac 2 strip_tac \\ first_x_assum drule
+  \\ fs [code_rel_def] \\ disch_then drule \\ fs []);
 
 
 
